graph/marked_graph.v
@@ -770,7 +770,7 @@ Context {EV: EqDec V eq}.
 Context {EE: EqDec E eq}.
 Context {DV DE: Type}.
 Context {MGS: MarkGraphSetting DV}.
-Context {P: PreGraph V E -> (V -> DV) -> (E -> DE) -> Type}.
+Context {P: LabeledGraph V E DV DE -> Type}.
 
 Notation Graph := (GeneralGraph V E DV DE P).
 
@@ -794,8 +794,8 @@ Definition mark (g1 : Graph) (root : V) (g2 : Graph) : Prop :=
   (forall n, ~ g1 |= root ~o~> n satisfying (unmarked g1) -> (marked g1 n <-> marked g2 n)).
 
 Inductive mark_list: Graph -> list V -> Graph -> Prop :=
-| mark_list_nil: forall g g0, (g ~=~ g0)%GeneralGraph -> mark_list g nil g0
-| mark_list_cons: forall g g0 g1 v vs, mark g v g0 -> mark_list g0 vs g1 -> mark_list g (v :: vs) g1
+| mark_list_nil: forall (g g0: Graph), (g ~=~ g0)%LabeledGraph -> mark_list g nil g0
+| mark_list_cons: forall (g g0 g1: Graph) v vs, mark g v g0 -> mark_list g0 vs g1 -> mark_list g (v :: vs) g1
 .
 
 Definition inj (g: Graph): NodePred V.
@@ -803,7 +803,7 @@ Definition inj (g: Graph): NodePred V.
   intros; apply marked_dec.
 Defined.
 
-Instance inj_proper: Proper (general_graph_equiv ==> node_pred_equiv) inj.
+Instance inj_proper: Proper ((fun (g1 g2: Graph) => (g1 ~=~ g2)%LabeledGraph) ==> node_pred_equiv) inj.
 Proof.
   hnf; intros.
   intro; simpl.
@@ -938,7 +938,7 @@ Context {EV: EqDec V eq}.
 Context {EE: EqDec E eq}.
 Context {DV DE: Type}.
 Context {MGS: MarkGraphSetting DV}.
-Context {P: PreGraph V E -> (V -> DV) -> (E -> DE) -> Type}.
+Context {P: LabeledGraph V E DV DE -> Type}.
 
 Notation Graph := (GeneralGraph V E DV DE P).
 
@@ -978,8 +978,8 @@ Definition mark (g1 : Graph) (root : V) (g2 : Graph) : Prop :=
   (forall n, ~ g1 |= root ~o~> n satisfying (unmarked g1) -> (marked g1 n <-> marked g2 n)).
 
 Inductive mark_list: Graph -> list V -> Graph -> Prop :=
-| mark_list_nil: forall g g0, (g ~=~ g0)%GeneralGraph -> mark_list g nil g0
-| mark_list_cons: forall g g0 g1 v vs, mark g v g0 -> mark_list g0 vs g1 -> mark_list g (v :: vs) g1
+| mark_list_nil: forall (g g0: Graph), (g ~=~ g0)%LabeledGraph -> mark_list g nil g0
+| mark_list_cons: forall (g g0: Graph) g1 v vs, mark g v g0 -> mark_list g0 vs g1 -> mark_list g (v :: vs) g1
 .
 
 Definition inj (g: Graph): NodePred V.
@@ -987,7 +987,7 @@ Definition inj (g: Graph): NodePred V.
   intros; apply marked_dec.
 Defined.
 
-Instance inj_proper: Proper (general_graph_equiv ==> node_pred_equiv) inj.
+Instance inj_proper: Proper ((fun (g1 g2: Graph) => (g1 ~=~ g2)%LabeledGraph) ==> node_pred_equiv) inj.
 Proof.
   hnf; intros.
   intro; simpl.
