graph/spanning_tree.v
@@ -443,7 +443,7 @@ Section SPANNING.
   Context {EE: EqDec E eq}.
   Context {DV DE: Type}.
   Context {MGS: MarkGraphSetting DV}.
-  Context {P: PreGraph V E -> (V -> DV) -> (E -> DE) -> Type}.
+  Context {P: LabeledGraph V E DV DE -> Type}.
   Notation Graph := (GeneralGraph V E DV DE P).
 
   Definition is_tree (g : PreGraph V E) (x : V) : Prop := SIMPLE_SPANNING_TREE.is_tree g x.
@@ -565,7 +565,7 @@ Section SPANNING.
   Qed.
 
   Inductive spanning_list : Graph -> list E -> Graph -> Prop :=
-  | spanning_list_nil: forall (g1 g2 : Graph), g1 ~=~ g2%GeneralGraph -> spanning_list g1 nil g2
+  | spanning_list_nil: forall (g1 g2 : Graph), g1 ~=~ g2%LabeledGraph -> spanning_list g1 nil g2
   | spanning_list_cons:
       forall g1 g2 g3 e rest, edge_spanning_tree g1 e g2 -> spanning_list g2 rest g3 -> spanning_list g1 (e :: rest) g3.
 
